\begin{equation}
  \begin{aligned}
    \va{F} &= F_1\hat{e_x} + F_2\hat{e_r} + F_3\hat{e_\phi} \\
    \pdv{\va{F}}{x} &= 
    \pdv{F_1}{x}\hat{e_x} + 
    \pdv{F_2}{x}\hat{e_r} + 
    \pdv{F_3}{x}\hat{e_\phi} \\
    \pdv{\va{F}}{r} &= 
    \pdv{F_1}{r}\hat{e_x} + 
    \pdv{F_2}{r}\hat{e_r} + 
    \pdv{F_3}{r}\hat{e_\phi} \\
    \pdv{\va{F}}{\phi} &= 
    \pdv{F_1}{\phi}\hat{e_x} + 
    \left(\pdv{F_2}{\phi} - F_3\right)\hat{e_r} + 
    \left(\pdv{F_3}{\phi} + F2\right)\hat{e_\phi}
  \end{aligned}
\end{equation}
